Progress on Spec.UPKE

specs/experimental/Spec.UPKE.fst
@@ -14,6 +14,11 @@ module HKDF = Spec.Agile.HKDF
 module HPKE = Spec.HPKE
 
 
+/// Clamp(a)
+
+assume val of_string: string -> bytes
+assume val scalar_to_nat: alg:DH.algorithm -> DH.scalar alg -> nat
+assume val nat_to_scalar: alg:DH.algorithm -> nat -> DH.scalar alg
 
 /// Mult(a,b) {
 ///   c = (Clamp(a) * Clamp(b)) mod order
@@ -21,6 +26,17 @@ module HPKE = Spec.HPKE
 ///     c = (order - c) mod order
 ///   return c
 /// }
+
+val mul: alg:DH.algorithm -> DH.scalar alg -> DH.scalar alg -> Tot nat
+let mul alg a b =
+  let (a, b) = match alg with
+    | DH.DH_Curve25519 -> (DH.clamp alg a, DH.clamp alg b)
+    | DH.DH_Curve448 -> (DH.clamp alg a, DH.clamp alg b)
+    | DH.DH_P256 -> (a, b) in
+  let c = ((scalar_to_nat alg a) * (scalar_to_nat alg b)) % (DH.order alg) in
+  // BB. Missing a reduction if the msb is = 0 because I can't quickly
+  //     implement it in constant time.
+  c
 
 
 /// UPKE-Encrypt(pk, m):
@@ -31,6 +47,22 @@ module HPKE = Spec.HPKE
 ///   pk' := DH(pk, d)
 ///   return ((c1, c2), pk')
 
+val encrypt:
+    cs:HPKE.ciphersuite
+  -> deltaE:bytes
+  -> skE:HPKE.key_dh_secret_s cs
+  -> pkR:HPKE.key_dh_public_s cs
+  -> m:bytes ->
+  Tot(HPKE.key_dh_public_s cs & bytes & HPKE.key_dh_public_s cs)
+
+let encrypt cs deltaE skE pkR m =
+  let delta = HKDF.expand (HPKE.hash_of_cs cs) deltaE (of_string "derive UPKE delta") (HPKE.size_dh_key cs) in
+  let pkE,k,n = HPKE.setupBaseI cs skE pkR bytes_empty in
+  let content = Seq.append deltaE m in
+  let c = AEAD.aead_encrypt (HPKE.aead_of_cs cs) k n content lbytes_empty in
+  let pkR' = DH.scalarmult (HPKE.curve_of_cs cs) delta pkR in
+  pkE,c,pkR'
+
 
 /// UPKE-Decrypt(sk, (c1, c2)):
 ///   epk, context := HPKE.SetupBaseR(c1, sk, "")
@@ -38,3 +70,23 @@ module HPKE = Spec.HPKE
 ///   d := HKDF(sksize, d', "", "derive UPKE delta")
 ///   sk' := Mult(sk, d)
 ///   return (m, sk')
+
+val decrypt:
+    cs:HPKE.ciphersuite
+  -> pkE:HPKE.key_dh_public_s cs
+  -> skR:HPKE.key_dh_secret_s cs
+  -> ct:bytes ->
+  Tot(option (bytes & HPKE.key_dh_secret_s cs))
+
+let decrypt cs pkE skR ct =
+  let k,n = HPKE.setupBaseR cs pkE skR bytes_empty in
+  let c = Seq.slice ct 0 (Seq.length ct - (AEAD.size_tag (HPKE.aead_of_cs cs))) in
+  let tag = Seq.slice ct (Seq.length ct - (AEAD.size_tag (HPKE.aead_of_cs cs))) (Seq.length ct) in
+  match AEAD.aead_decrypt (HPKE.aead_of_cs cs) k n c tag lbytes_empty with
+  | None -> None
+  | Some p ->
+  let deltaE = Seq.slice p (HPKE.size_dh_key cs) (Seq.length p - (HPKE.size_dh_key cs)) in
+  let m = Seq.slice p (Seq.length p - (HPKE.size_dh_key cs)) (Seq.length p) in
+  let delta = HKDF.expand (HPKE.hash_of_cs cs) deltaE (of_string "derive UPKE delta") (HPKE.size_dh_key cs) in
+  let skR' = DH.scalarmult (HPKE.curve_of_cs cs) skR delta in
+  Some (m, skR')
